sigpred: qed irrefutable evidence lemmas

proof/ktcore_proof/sigpred.v
@@ -10,23 +10,9 @@ From New.proof.github_com.sanjit_bhat.pav.ktcore_proof Require Import
 Module ktcore.
 Import key_map.ktcore serde.ktcore.
 
-(*
-to refresh, structure of digs pred:
-- there's a mono_list of digs.
-mono is important. means that two sigs at diff epochs overlap.
-- auditor gets starting link at some StartEpoch.
-invert with fuel:=StartEpoch to get some digs.
-when inverting, could fewer digs than StartEpoch.
-could invert to cut.
+Module sigpred.
 
-reqs:
-- need to state that maps are mono.
-but which maps? hidden or plain?
-- from hidden mono, can derive plain mono.
-so let's do that.
-*)
-
-Module sigpred_cfg.
+Module cfg.
 Record t :=
   mk {
     vrf : gname;
@@ -40,50 +26,85 @@ Record t :=
     (* the offset in digs after which auditor started monitoring. *)
     audit_offset : gname;
   }.
-End sigpred_cfg.
+End cfg.
 
 Section proof.
 Context `{hG: heapGS Σ, !ffi_semantics _ _}.
-Context {sem : go.Semantics} {package_sem : ktcore.Assumptions}.
-Collection W := sem + package_sem.
+Context {sem : go.Semantics}.
+Collection W := sem.
 #[local] Set Default Proof Using "W".
 
-Definition sigpred_vrf γ (vrfPk : list w8) : iProp Σ :=
-  "#Hshot" ∷ dghost_var γ.(sigpred_cfg.vrf) (□) vrfPk.
+(** VRF sig. *)
 
-Definition sigpred_vrf_aux γ enc : iProp Σ :=
+Definition vrfP γ (vrfPk : list w8) : iProp Σ :=
+  "#Hshot" ∷ dghost_var γ.(cfg.vrf) (□) vrfPk.
+
+Definition vrfP_aux γ enc : iProp Σ :=
   ∃ vrfPk,
   "%Henc" ∷ ⌜enc = ktcore.VrfSig.pure_enc (ktcore.VrfSig.mk' (W8 ktcore.VrfSigTag) vrfPk)⌝ ∗
   "%Hvalid" ∷ ⌜safemarshal.Slice1D.valid vrfPk⌝ ∗
-  "#Hsigpred" ∷ sigpred_vrf γ vrfPk.
+  "#Hsigpred" ∷ vrfP γ vrfPk.
 
-Definition digs_mono digs audit_offset :=
+Lemma vrfP_evid γ vrfPk0 vrfPk1 :
+  vrfP γ vrfPk0 -∗
+  vrfP γ vrfPk1 -∗
+  ⌜vrfPk0 = vrfPk1⌝.
+Proof.
+  rewrite /vrfP. iNamedSuffix 1 "0". iNamedSuffix 1 "1".
+  by iCombine "Hshot0 Hshot1" gives %[_ ->].
+Qed.
+
+(** Link sig. *)
+
+Definition mono digs audit_offset :=
   let hidden_maps := merkle.inv_fn <$> digs in
   (* ⊆ on hidden maps is stronger than on plain maps. *)
   list_reln (drop audit_offset hidden_maps) (⊆).
 
-Definition sigpred_link γ (ep : w64) link : iProp Σ :=
+Definition linkP γ (ep : w64) link : iProp Σ :=
   ∃ start_ep audit_offset,
   let '(digs, cut) := hashchain.inv_fn link (S $ S $ uint.nat ep) in
-  "#Hlb_digs" ∷ mono_list_lb_own γ.(sigpred_cfg.digs) digs ∗
-  "#His_start" ∷ dghost_var γ.(sigpred_cfg.start_ep) (□) start_ep ∗
+  "#Hlb_digs" ∷ mono_list_lb_own γ.(cfg.digs) digs ∗
+  "#His_start" ∷ dghost_var γ.(cfg.start_ep) (□) start_ep ∗
   "%Hlen_digs" ∷ ⌜S $ uint.nat ep = (start_ep + length digs)%nat⌝ ∗
-  "#His_cut" ∷ dghost_var γ.(sigpred_cfg.cut) (□) cut ∗
-  "#His_offset" ∷ dghost_var γ.(sigpred_cfg.audit_offset) (□) audit_offset ∗
-  "%Hmono" ∷ ⌜digs_mono digs audit_offset⌝.
+  "#His_cut" ∷ dghost_var γ.(cfg.cut) (□) cut ∗
+  "#His_offset" ∷ dghost_var γ.(cfg.audit_offset) (□) audit_offset ∗
+  "%Hmono" ∷ ⌜mono digs audit_offset⌝.
 
-Definition sigpred_link_aux γ enc : iProp Σ :=
+Definition linkP_aux γ enc : iProp Σ :=
   ∃ ep link,
   "%Henc" ∷ ⌜enc = ktcore.LinkSig.pure_enc (ktcore.LinkSig.mk' (W8 ktcore.LinkSigTag) ep link)⌝ ∗
   "%Hvalid" ∷ ⌜safemarshal.Slice1D.valid link⌝ ∗
-  "#Hsigpred" ∷ sigpred_link γ ep link.
+  "#Hsigpred" ∷ linkP γ ep link.
 
-Definition sigpred γ enc : iProp Σ :=
-  sigpred_vrf_aux γ enc ∨ sigpred_link_aux γ enc.
+Definition P γ enc : iProp Σ :=
+  vrfP_aux γ enc ∨ linkP_aux γ enc.
 
-#[global] Instance sigpred_pers γ e : Persistent (sigpred γ e).
+#[global] Instance P_pers γ e : Persistent (P γ e).
 Proof. apply _. Qed.
 
+Lemma linkP_evid γ ep link0 link1 :
+  linkP γ ep link0 -∗
+  linkP γ ep link1 -∗
+  ⌜link0 = link1⌝.
+Proof.
+  rewrite /linkP. iIntros "H0 H1".
+  iNamed "H0". iNamed "H1".
+  case_match eqn:Hinv0.
+  case_match eqn:Hinv1.
+  iNamedSuffix "H0" "0". iNamedSuffix "H1" "1".
+  iCombine "His_start0 His_start1" gives %[_ ->].
+  iCombine "His_cut0 His_cut1" gives %[_ ->].
+  iDestruct (mono_list_lb_valid with "Hlb_digs0 Hlb_digs1") as %Hpref.
+  assert (l = l0) as ->.
+  { assert (length l = length l0) by word.
+    destruct Hpref as [Ht|Ht];
+      (apply prefix_length_eq in Ht; [done|lia]). }
+  opose proof (hashchain.det link0 link1 _ _ _) as ->; [|done].
+  erewrite Hinv0. by erewrite Hinv1.
+Qed.
+
+(*
 Lemma sigpred_links_inv_grow start_ep links link digs dig cut maps m :
   (∀ prev_map, last maps = Some prev_map → prev_map ⊆ m) →
   sigpred_links_inv start_ep links digs cut maps -∗
@@ -123,6 +144,8 @@ Proof.
       + done. }
   { iPureIntro. by apply list_reln_snoc. }
 Qed.
+*)
 
 End proof.
+End sigpred.
 End ktcore.
